Foundation/Meta/ClProver.lean
@@ -84,7 +84,7 @@ structure Context where
   LC : Q(LogicalConnective $F)
   DC : Q(DecidableEq $F)
   S : Q(Type levelS)
-  E : Q(Entailment.{_, _, levelE} $F $S)
+  E : Q(Entailment.{_, _, levelE} $S $F)
   𝓢 : Q($S)
   CL : Q(Entailment.Cl $𝓢)
 
@@ -347,7 +347,7 @@ structure HypInfo where
   levelE : Level
   F : Q(Type levelF)
   S : Q(Type levelS)
-  E : Q(Entailment.{_, _, levelE} $F $S)
+  E : Q(Entailment.{_, _, levelE} $S $F)
   𝓢 : Q($S)
   φ : Q($F)
   proof : Q($𝓢 ⊢ $φ)
